Attempts at advanced

src/inductive/IG.v
@@ -106,8 +106,7 @@ Definition _cleanSplit {A B : Type} (node : Node) (context' : Context' A B) (ig 
     
     let ig' := _updAdj froms' (fun x y => _clearSucc node y) ig in 
     let ig'' := _updAdj tos' (fun x y => _clearPred node y) ig' in
-    (context, ig'')
-    .
+    (context, ig'').
 
 
 Definition IG_match {A B : Type} (node : Node) (ig : IG A B) : Decomp A B :=
@@ -135,6 +134,9 @@ Definition IG_and {A B : Type} (context : Context A B) (ig : IG A B) : IG A B :=
     let ig'' := _updAdj tos (_addPred node) ig' in
     _updAdj froms (_addSucc node) ig''.
 
+Notation "c I& ig" := (IG_and c ig) (at level 59, right associativity). 
+
+
 
 Definition _insNode {A B : Type} (node : LNode A) (ig : IG A B) : IG A B :=
     let '(n, l) := node in
@@ -142,7 +144,6 @@ Definition _insNode {A B : Type} (node : LNode A) (ig : IG A B) : IG A B :=
 
 Definition _insNodes {A B : Type} (nodes : list (LNode A)) (ig : IG A B) : IG A B :=
     fold_right _insNode ig nodes.
-
 
 
 Definition _insEdge {A B : Type} (edge : LEdge B) (ig : IG A B) : IG A B :=
