src/inductive/IG_going_further_theory.v
@@ -59,17 +59,58 @@ Admitted.
 Lemma matchAnyIsAdd : forall (A B : Type) (ig i : IG A B) (c : Context A B),
     IG_matchAny ig = (Some c,  i) -> ig I== IG_and c i.
 Proof.
-    intros. unfold IG_equiv.
-    unfold IG_matchAny in H.
-Admitted.
+    intros. unfold IG_matchAny in H.
+    destruct (IG_labNodes ig).
+    - inversion H.
+    - eapply matchIsAdd. apply H.
+Qed.
 
 
-(* 
 
-Instance Proper_add {A B : Type} : Proper ((@contextEquiv A B) ==> (@IG_equiv A B) ==> (@IG_equiv A B)) IG_and. 
+
+
+
+
+
+
+
+
+(* Some of this is duplicated *)
+Instance IG_Equivalence {A B : Type} : Equivalence (@IG_equiv A B).
+Proof.
+    G_derived_equivalence_prover nat unit (@ IG_to_RG A B).  
+Qed.
+
+Definition contextEquiv {A B : Type} (c1 c2 : Context A B) : Prop :=
+    c1 = c2.
+
+
+
+(* This one is really hard... *)
+Instance Proper_and {A B : Type} : Proper ((@contextEquiv A B) ==> (@IG_equiv A B) ==> (@IG_equiv A B)) (IG_and).  
 Proof.
 Admitted. 
 
+
+
+
+
+(* Doable with some induction probably *)
+Lemma IG_matchAny_None_is_empty : forall (A B : Type) (ig i : IG A B),
+    IG_matchAny ig = (None, i) -> IG_isEmpty ig = true.
+Proof.
+Admitted.
+
+(* Doable with some lemmas probably *)
+Lemma IG_isEmpty_equiv_empty : forall (A B : Type) (ig : IG A B),
+    IG_isEmpty ig = true <-> ig I== IG_empty.
+Proof.
+Admitted.
+
+
+(* Relies on unproven lemmas:
+Proper_and
+... *)
 Lemma IG_ufold_nothing : forall (A B : Type) (ig : IG A B),
     IG_ufold _ _ _ IG_and IG_empty ig I== ig.
 Proof.
@@ -82,23 +123,21 @@ Proof.
     rewrite IG_ufold_equation.
     destruct (IG_matchAny ig) eqn:mat.
     destruct m eqn:mm.
-    - specialize (IH i). assert (ltof (IG A B) IG_noNodes i ig). {
-        unfold ltof.
-        apply _IG_matchAny_decreases_IG_noNodes in mat.
-        assumption.
-        }
-        specialize (IH H). clear H.
+    (* The "smaller" graph I use for IH is i *) 
+    - specialize (IH i). apply _IG_matchAny_decreases_IG_noNodes in mat as mat'. unfold ltof in IH.
+        specialize (IH mat'). clear mat'.
+
         rewrite IH.
         apply matchAnyIsAdd in mat. rewrite <- mat. reflexivity.
 
-    -  
-    
-    admit. (*easy*)
-Admitted.
+    - apply IG_matchAny_None_is_empty in mat. apply IG_isEmpty_equiv_empty in mat.
+        rewrite mat. reflexivity.
+Qed.
 
 
 
 
+(* ERelies on unproved Proper_and *)
 Lemma IG_ufold_add : forall (A B : Type)  (c : Context A B) (ig : IG A B),
     IG_ufold _ _ _ IG_and IG_empty (IG_and c ig) I== IG_and c (IG_ufold _ _ _ IG_and IG_empty ig).
 Proof.
@@ -119,21 +158,25 @@ Lemma IG_ufold_rec :
     forall (A B C : Type) (P : IG A B -> C -> Prop) (f : Context A B -> C -> C),
         forall (i : C) (g : IG A B), 
         (forall g, IG_isEmpty g = true -> P g i) -> 
-        (forall k a g' g'', (_key_In_IG k ( g))) -> ~ (_key_In_IG k ( g'))) -> 
-        match IG_match k g with
-        | (Some context, rest) => P g' (f context a) -> P g'' (f context a)
-        | _ => False
-        end) ->
+
+        (forall k c any a g' g'', IG_match k g = (Some c, any) -> ~_key_In_IG k g' ->
+        g' I== IG_and c g'' -> P g' a -> P g'' (f c a)) ->
+
 
         P g (IG_ufold _ _ _ f i g).
 Proof.
     intros.
 Admitted.
 
-(* This is probably true, but does not really work in my case *)
-(* This can make it to the final thesism however relies on an unfinished lemma *)
-Lemma IG_induction : forall (A B : Type) g (P : IG A B -> Prop) (rewriteP : Proper (IG_equiv ==> eq) P),
-    P IG_empty -> (forall g c, P g -> P (IG_and c g)) ->
+
+
+(* This depends on these lemmas to be true:
+IG_matchAny_None_is_empty
+IG_isEmpty_equiv_empty
+matchAnyIsAdd
+*)
+Lemma IG_induction : forall (A B : Type) (g : IG A B) (P : IG A B -> Prop) (rewriteP : Proper (IG_equiv ==> eq) P),
+    P IG_empty -> (forall g' c, P g' -> P (IG_and c g')) ->
     P g.
 Proof.
     intros A B ig P rewriteP base IH.
@@ -144,72 +187,743 @@ Proof.
     destruct m eqn:mm.
     - subst. specialize (IH i c).
         apply matchAnyIsAdd in mat as isAdd.
-        subst.
-        apply IH.
-        specialize (H i).
+        rewrite (rewriteP _ _ isAdd).
+        apply IH. 
         apply H.
+
         apply _IG_matchAny_decreases_IG_noNodes in mat.
-        unfold ltof. auto.
+        unfold ltof. assumption.
     (* No hit: *)
-        - unfold IG_matchAny in mat. destruct (IG_labNodes x) eqn:labNodes.
-        + inversion mat. subst. unfold IG_labNodes in labNodes.
-        apply map_eq_nil in labNodes.
-        apply MProps.elements_Empty in labNodes.
-        assert (NatMap.Equal i IG_empty). {
-            unfold IG_empty.
-            unfold NatMap.Equal.
-            intros.
-            Search NatMap.find.
-            rewrite MFacts.empty_o.
-            apply MFacts.not_find_in_iff.
-            unfold not. intros.
-            Search NatMap.In.
-            unfold NatMap.Empty in labNodes.
-            unfold NatMap.In in H0.
-            admit.
-        }
-        destruct (rewriteP i IG_empty). 
-        -- admit.
-        -- assumption.
-
-        + unfold IG_match in mat. destruct (NatMap.find (fst l) x) eqn:found.
-        -- destruct (_cleanSplit (fst l) c (NatMap.remove (elt:=Context' A B) (fst l) x)).
-            inversion mat.
-        -- assert (x = IG_empty). {
-            admit.
-            }
-            rewrite H0.
-            assumption.
-Admitted.
+    - apply IG_matchAny_None_is_empty in mat. apply IG_isEmpty_equiv_empty in mat.
+        rewrite (rewriteP _ _ mat). assumption.
+Qed.
 
 
 
-Lemma _matchAny_add_IG_empty : forall (A B : Type) (c hit : Context A B) (i : IG A B),
-    IG_matchAny (IG_and c IG_empty) = (Some hit, i)
-    -> let '(froms, node, label, tos) := c in IG_isEmpty i = true /\ hit = ([], node, label, []).
+
+
+
+
+
+
+
+
+
+
+
+
+
+
+
+
+
+
+
+
+
+
+
+
+
+
+
+
+
+
+
+
+
+
+
+
+
+
+
+
+
+Instance Proper_RG_and {A B : Type} : Proper ((@contextEquiv A B) ==> (@RG_equiv nat unit) ==> (@RG_equiv nat unit)) RG_and. 
 Proof.
-Admitted.
+    split; unfold contextEquiv in H; subst; destruct y as [[[froms node] label] tos].
+    - firstorder.
+    - firstorder.
+Qed.
+
 
 
 Lemma IG_to_RG_distributes_over_add_using_IG_induction : forall {A B : Type} (c : Context A B) (ig : IG A B),
     IG_to_RG (IG_and c ig) R== RG_and c (IG_to_RG ig). 
 Proof.
     intros.
-    unfold IG_to_RG at 2.
-    apply (IG_ufold_rec A B). 
-    - admit. (* Here, I need some thinking *)
-    - intros. unfold IG_to_RG.
-    rewrite !IG_ufold_equation.
+    generalize dependent c.
+    apply (IG_induction A B ig (fun ig => forall c : Context A B, IG_to_RG (IG_and c ig)
+R== RG_and c (IG_to_RG ig))). 
+    - admit. (* Doable *)
+    - admit. (* Doable *)
+    - intros. rewrite H . (* Does not help *)
+Admitted.
+
+
+
+Lemma IG_to_RG_distributes_over_add_using_openign_defs : forall {A B : Type} (c : Context A B) (ig : IG A B),
+    IG_to_RG (IG_and c ig) R== RG_and c (IG_to_RG ig). 
+Proof.
+    intros.
+    generalize dependent c.
+    apply (IG_induction A B ig (fun ig => forall c : Context A B, IG_to_RG (IG_and c ig)
+R== RG_and c (IG_to_RG ig))). 
+    - admit. (* Doable *)
+    - admit. (* Doable *)
+    - intros. rewrite H . (* Does not help *)
+Admitted.
+
+
+
+
+
+
+
+
+
+
+
+
+
+
+
+
+
+
+
+(* New model to show transpose *)
+
+
+
+Require Import GraphVerification.src.inductive.IG_theory.
+Require Import GraphVerification.src.inductive.IG_wf_algorithms_theory.
+
+Lemma IG_to_RG'_valid : forall (A B : Type) (ig : IG A B),
+_valid_cond (fun n : nat => _key_In_IG n ig)
+(fun (n1 n2 : nat) (_ : unit) => exists l : B, In (n1, n2, l) (IG_labEdges ig)).
+Proof.
+Admitted.
+
+Definition IG_to_RG' {A B : Type} (ig : IG A B) : RG_unlE nat.
+Proof.
+    refine {|
+        RG_nodes := fun (n : nat) => _key_In_IG n ig;
+        RG_edges := fun (n1 n2 : nat) l => exists l, In (n1, n2, l) (IG_labEdges ig);
+        RG_valid := _
+    |}.
+    apply IG_to_RG'_valid. (* Bypass*)
+Defined.
+
+
+
+
+
+
+Lemma IG_to_RG_distributes_over_add' : forall {A B : Type} (c : Context A B) (ig : IG A B),
+    IG_to_RG' (IG_and c ig) R== RG_and c (IG_to_RG' ig). 
+Proof.
+Admitted.
+
+
+
+
+
+
+
+
+
+
+
+Theorem IG_transpose_is_RG : forall (A B : Type) (ig : IG A B),
+    IG_to_RG' (IG_transpose ig) R== RG_transpose (IG_to_RG' ig).
+Proof.
+    intros A B.
+    apply (well_founded_induction (well_founded_ltof _ IG_noNodes)).
+    intros ig IH.
+    unfold IG_transpose. unfold IG_gmap.
+    unfold IG_to_RG.
+    rewrite !IG_ufold_equation. destruct (IG_matchAny ig) eqn:mat.
+    destruct m.
+    - specialize (IH i).
+        apply _IG_matchAny_decreases_IG_noNodes in mat as mat'.
+        specialize (IH mat').
+        (* This one is not fully proven *)
+        rewrite IG_to_RG_distributes_over_add'.
+        rewrite -> IH.
+        rewrite <- RG_transpose_distributes_over_extendByContext.
+        (* Now, I somehow need to show that if I have a match, I can derive a I& from it *)
+         
+Admitted.
+(*      
+        Check RG_transpose_distributes_over_extendByContext.
+        Check IG_to_RG_distributes_over_add'.
+        rewrite IG_to_RG_distributes_over_add'.
+        rewrite -> IH.
+        reflexivity.
+
+    - clear mat IH. unfold IG_to_RG. rewrite IG_ufold_equation. simpl. firstorder. 
+Qed. *)
+
+Theorem IG_transpose_is_RG_using_own_induction : forall (A B : Type) (ig : IG A B),
+    IG_to_RG' (IG_transpose ig) R== RG_transpose (IG_to_RG' ig).
+Proof.
+    intros.
+    apply (IG_induction A B ig (fun ig => IG_to_RG' (IG_transpose ig) R== RG_transpose (IG_to_RG' ig))).
+    - admit.
+    - firstorder.
+    - intros.
+        (* I can't continue here, since there is the problem, that I& does not really enforce any order, so one cannot distribute over it *)
+Admitted. 
+
+
+
+
+
+
+
+
+
+
+
+(* Now, I conider the smaller problem of showing that the nodes of I& are the same as the nodes of R& *)
+
+Lemma get_nodes_is_get_nodes : forall (A B : Type) (ig : IG A B) n,
+    _key_In_IG n ig <-> (IG_to_RG ig).(RG_nodes) n.
+Proof.
+    intros.
+    unfold IG_to_RG.
+    rewrite IG_ufold_equation.
+    destruct (IG_matchAny ig) eqn:mat.
+    destruct m.
+    - Admitted. 
+
+Require Import GraphVerification.src.util.util.
+
+
+
+
+
+
+Lemma helper_ufold_preserves_mem : forall (A B : Type) (node : Node) (ig : IG A B),
+    NatMap.mem node ig = true
+    <-> RG_nodes (IG_ufold A B (RG_unlE nat) RG_and RG_empty ig) node.
+Proof.
+    intros A B n.
+    
+    apply (well_founded_induction (well_founded_ltof _ (@IG_noNodes A B))).
+    intros ig IH.
+
+
+    rewrite IG_ufold_equation.
+    destruct (IG_matchAny ig) eqn:mat.
+    destruct m.
+    - specialize (IH i).
+        apply _IG_matchAny_decreases_IG_noNodes in mat as mat'.
+        specialize (IH mat').
+
+        destruct_context c. simpl. bdestruct (n =? node).
+        + subst. assert (NatMap.mem node ig = true). {
+            unfold IG_matchAny in mat. destruct (IG_labNodes ig).
+            - inversion mat.
+            - clear mat'. destruct l. simpl in *. apply IG_match_returns_node in mat as mat'. subst.
+                apply MFacts.mem_in_iff.
+
+
+
+
+                apply (IG_match_removes_node _ _ node) in mat as mat'.
+                apply (IG_match_exactly_removes_node _ _ _ _ _ _ (node, label)) in mat.
+                simpl in *.
+
+                apply NatMap_In_exists_MapsTo_iff.
+                rewrite _In_labNodes_is_some_MapsTo in mat.
+                clear IH.
+                assert ((node, label) = (node, label) /\ ~ _key_In_IG node i \/ In (node, label) (IG_labNodes i)). {
+                    left. auto. 
+                }
+                apply mat in H.
+                destruct_eMapsTo H.
+                exists (efroms, label, etos).
+                assumption.
+        }
+        rewrite H. unfold Ensemble_add. split; intros.
+        -- left. reflexivity.
+        -- reflexivity.
+    + unfold Ensemble_add. rewrite <- IH.
+        unfold IG_matchAny in mat. destruct (IG_labNodes ig).
+         -- inversion mat.
+         -- rewrite <- !MFacts.mem_in_iff.
+            rewrite !NatMap_In_exists_MapsTo_iff.
+            split; intros.
+            ++ destruct H0. destruct_context' x.
+                apply (IG_match_exactly_removes_node _ _ _ _ _ _ (n, label')) in mat.
+                rewrite !_In_labNodes_is_some_MapsTo in mat.
+                assert (exists froms tos : Adj B, NatMap.MapsTo n (froms, label', tos) ig). {
+                    exists froms', tos'. assumption. 
+                }
+
+                apply mat in H1. destruct H1.
+                --- destruct H1. inversion H1. rewrite H4 in H. unfold not in H. exfalso. apply H. reflexivity.
+                --- right. destruct_eMapsTo H1. exists (efroms, label', etos). assumption.
+            ++ destruct H0.
+                --- subst. exfalso. apply H. reflexivity.
+                --- destruct H0. destruct_context' x.
+                
+                
+                apply (IG_match_exactly_removes_node _ _ _ _ _ _ (n, label')) in mat.
+                rewrite !_In_labNodes_is_some_MapsTo in mat.
+                assert ((n, label') = (node, label) /\ ~ _key_In_IG (fst (n, label')) i \/ exists froms tos : Adj B, NatMap.MapsTo n (froms, label', tos) i). {
+                    right. exists froms', tos'. assumption. 
+                }
+                apply mat in H1. destruct_eMapsTo H1. exists (efroms, label', etos). assumption.
+    - apply IG_matchAny_None_is_empty in mat.
+        admit.
+Admitted.
+    
+    
+Lemma node_is_ins_added_node : forall (A B : Type) (c : Context A B) (ig : IG A B),
+    let '(froms, node, label, tos) := c in
+    RG_nodes (IG_to_RG (_updAdj froms (_addSucc node) (_updAdj tos (_addPred node)
+            (NatMap.add node (froms, label, tos) ig)))) node.
+Proof.
+    intros. destruct_context c.
+
+    apply (IG_induction A B ig (fun ig => RG_nodes (IG_to_RG (_updAdj froms (_addSucc node) (_updAdj tos (_addPred node)
+(NatMap.add node (froms, label, tos) ig)))) node)).
+
+    - admit.
+    - admit.
+    - intros. destruct_contextt c. bdestruct (node =? nodee).
+        + subst. 
+
+
+Admitted.
+
+(* Same as above, but now onIG_to_RG'. This is provable *)
+Lemma node_is_ins_added_node' : forall (A B : Type) (c : Context A B) (ig : IG A B),
+    let '(froms, node, label, tos) := c in
+    RG_nodes (IG_to_RG' (_updAdj froms (_addSucc node) (_updAdj tos (_addPred node)
+            (NatMap.add node (froms, label, tos) ig)))) node.
+Proof.
+    intros. destruct_context c. simpl.
+    unfold _key_In_IG. exists label.
+    apply _updAdj_addSucc_does_not_change_IG_labNodes.
+    apply _updAdj_addPred_does_not_change_IG_labNodes.
+    apply _In_labNodes_is_some_MapsTo.
+    exists froms, tos.
+    simpl.
+    apply MFacts.add_mapsto_iff.
+    auto.
+Qed.
+
+
+
+
+
+(* I tried reall hard to get this to work. It is essentially a sub-problem of relating I& to R&, but it is also dam hard *)
+Lemma get_nodes_is_get_nodes' : forall (A B : Type) (ig : IG A B) (c : Context A B) n,
+    (RG_and c (IG_to_RG ig)).(RG_nodes) n
+    <-> (IG_to_RG (IG_and c ig)).(RG_nodes) n.
+Proof.
+    intros.
+    unfold IG_and.
+    destruct_context c. simpl. unfold Ensemble_add.
+    destruct (NatMap.mem node ig) eqn:cond.
+    - split; intros.
+        + destruct H.
+            -- subst. admit. (* This semi proven *)
+            (* apply helper_ufold_preserves_mem in cond. assumption.   *)
+    
+            -- assumption.
+        + auto.
+    - bdestruct (n =? node).
+        -- subst. assert (RG_nodes (IG_to_RG (_updAdj froms (_addSucc node) (_updAdj tos (_addPred node)
+            (NatMap.add node (froms, label, tos) ig)))) node). {
+
+                        admit.
+            } split; intros.
+            ++ assumption.
+            ++ left. reflexivity.
+        -- split; intros.
+            ++ destruct H0.
+                --- subst. exfalso. apply H. reflexivity.
+                --- admit.
+            ++ right. admit.
+
+
+Admitted. 
+
+
+
+
+
+
+
+
+Lemma get_nodes_is_get_nodes''' : forall (A B : Type) (ig : IG A B) (c : Context A B) n,
+    (RG_and c (IG_to_RG' ig)).(RG_nodes) n
+    <-> (IG_to_RG' (IG_and c ig)).(RG_nodes) n.
+Proof.
+    intros.
+    unfold IG_and.
+    destruct_context c. simpl. unfold Ensemble_add.
+    destruct (NatMap.mem node ig) eqn:cond.
+    - split; intros.
+        + destruct H.
+            -- subst. admit. (* This semi proven *)
+            (* apply helper_ufold_preserves_mem in cond. assumption.   *)
+    
+            -- assumption.
+        + auto.
+    - bdestruct (n =? node).
+        -- subst. assert (RG_nodes (IG_to_RG (_updAdj froms (_addSucc node) (_updAdj tos (_addPred node)
+            (NatMap.add node (froms, label, tos) ig)))) node). {
+
+                        admit.
+            } split; intros.
+            ++ admit.
+            ++ left. reflexivity.
+        -- split; intros.
+            ++ destruct H0.
+                --- subst. exfalso. apply H. reflexivity.
+                --- admit.
+            ++ right. admit.
+
+
+Admitted. 
+
+
+
+
+
+
+
+
+
+
+
+
+
+
+
+
+
+
+
+
+
+
+
+
+
+
+
+
+
+
+
+
+
+
+
+
+
+
+
+
+
+
+
+(* Thinking about which operations are usable in a gmap *)
+
+
+Notation "c I& ig" := (IG_and c ig) (at level 59, right associativity).
+
+
+
+Definition _annihilate {A B : Type} (n : Node) (context : Context A B) : Context A B :=
+    let '(froms, node, label, tos) := context in
+    let c' := _clearPred n (froms, label, tos) in
+    let '(fromss, labell, toss) := _clearSucc n c' in
+    (fromss, node, labell, toss).
+
+Print Adj.
+
+Definition megaContext {A B : Type} (base extender : Context A B) : Context A B :=
+    let '(efroms, enode, elabel, etos) := extender in
+    let '(bfroms, bnode, blabel, btos) := base in
+    let fromExtender := map (fun '(l, n) => (l, enode)) (filter (fun '(_, n) => n =? bnode) etos) in
+    let toExtender := map (fun '(l, n) => (l, enode)) (filter (fun '(_, n) => n =? bnode) efroms) in
+    (bfroms ++ fromExtender, bnode, blabel, btos ++ toExtender).
+
+
+
+
+
+Lemma IG_and_semi_commutative : forall (A B : Type) (c1 c2 : Context A B) (ig : IG A B),
+    c1 I& c2 I& ig I== 
+            let '(_, node2, _, _) := c2 in
+        megaContext c2 c1 I& _annihilate node2 c1 I& ig.
+Proof.
+    intros.
+    
 
     
+    
+    destruct_context c1. destruct_contextt c2. simpl.
+    destruct (NatMap.mem nodee ig) eqn:cond1.
+    - destruct (NatMap.mem node ig) eqn:cond2.
+        + destruct (NatMap.mem nodee ig) eqn:cond3.
+            -- reflexivity.
+            -- inversion cond1.
+        + admit. (* I have no clue, why destruct, rewrite, remember do not work here *)
+        
+    - destruct (NatMap.mem (elt:=Context' A B) node
+(_updAdj fromss (_addSucc nodee) (_updAdj toss (_addPred nodee) (NatMap.add nodee (fromss, labell, toss) ig)))) eqn:cond2.
+        + destruct (NatMap.mem node ig) eqn:cond3.
+            -- destruct (NatMap.mem nodee ig) eqn:cond4.
+                ++ inversion cond1.
+                ++ admit. (* Here, there is work to do *)
+            -- admit. (* I have no clue, why destruct, rewrite, remember do not work here *)
+        + destruct (NatMap.mem node ig) eqn:cond3.
+            -- destruct (NatMap.mem nodee ig) eqn:cond4.
+                ++ inversion cond1.
+                ++ admit. (* Here, there is work to do *)
+            -- admit. (* I have no clue, why destruct, rewrite, remember do not work here *)
+
+Admitted.
+
+
+Check incl.
+Print incl.
+
+(* Characterizing the functions for which fold is universally correct *)
+
+Lemma IG_map_splits_when : forall (A B C D: Type) (f : Context A B -> Context C D) (c : Context A B) (ig : IG A B),
+    (forall anyC,
+    let '(froms, node, label, tos) := anyC in
+    let '(froms', node', label', tos') := f anyC in
+    let possibleNeighbours := map snd froms ++ map snd tos in
+    node = node' /\
+    incl (map snd froms') possibleNeighbours /\  
+    incl (map snd tos') possibleNeighbours)
+    
+    ->
+
+    IG_gmap f (c I& ig) I== f c I& IG_gmap f ig.
+Proof.
+    intros.
+    destruct_context c.
+Admitted.
+
+
+
+
+
+
+
+
+
+
+
+
+
+
+
+Definition _mappable_based_on_edge {A B : Type} (nStart nEnd : Node) (whatToDoBasedConnections : list (LEdge B) -> (Adj B * Adj B)) (c : Context A B) : Context A B :=  
+    let '(froms, node, label, tos) := c in
+    if node =? nEnd then
+        let listOfEdges := map (fun '(l, _) => (nStart, nEnd, l)) (filter (fun '(_, n) => n =? nStart) froms) in
+        let '(newFroms, newTos) := whatToDoBasedConnections listOfEdges in
+        (froms ++ newFroms, node, label, tos ++ newTos)
+    else
+        if node =? nStart then
+            let listOfEdges := map (fun '(l, _) => (nStart, nEnd, l)) (filter (fun '(_, n) => n =? nEnd) tos) in
+            let '(newFroms, newTos) := whatToDoBasedConnections listOfEdges in
+            (froms ++ newFroms, node, label, tos ++ newTos)
+            
+        else
+            c.
+Require Import Permutation.
+
+
+Lemma _mappable_based_on_edge_is_mappable : forall (A B : Type) (nStart nEnd : Node) (whatToDoBasedConnections : list (LEdge B) -> (Adj B * Adj B)) (c : Context A B) (ig1 ig2 : IG A B),
+
+    (forall (input : list (LEdge B)),
+    Forall (fun '(n1, n2, l) => nStart = n1 /\ nEnd = n2) input ->
+        let '(froms, tos) := whatToDoBasedConnections input in
+        Forall (fun '(l, n) => nStart = n \/ nEnd = n) froms /\ Forall (fun '(l, n) => nStart = n \/ nEnd = n) tos)
+
+    ->
+
+    (forall (input1 input2 : list (LEdge B)), Permutation input1 input2 ->
+        let '(froms1, tos1) := whatToDoBasedConnections input1 in
+        let '(froms2, tos2) := whatToDoBasedConnections input2 in
+        Permutation froms1 froms2 /\ Permutation tos1 tos2)
+    ->
+ 
+    ig1 I== ig2 ->
+    IG_gmap (fun c => _mappable_based_on_edge nStart nEnd whatToDoBasedConnections c) ig1
+    I== IG_gmap (fun c => _mappable_based_on_edge nStart nEnd whatToDoBasedConnections c) ig2.
+Proof.
+Admitted.
+
+
+
+
+
+
+Definition _rename_node_label {A B C : Type} (f : LNode A -> C) (c : Context A B) : Context C B :=
+    let '(froms, node, label, tos) := c in
+    (froms, node, f (node, label), tos).
+
+Lemma _rename_node_label_correct : forall (A B C : Type) (f : LNode A -> C) (ig1 ig2 : IG A B),
+    ig1 I== ig2
+    -> IG_gmap (fun c => _rename_node_label f c) ig1 I== IG_gmap (fun c => _rename_node_label f c) ig2.
+Proof.
+Admitted.
+
+
+
+
+
+Definition _rename_edge_label {A B C : Type} (f : LEdge B -> C) (c : Context A B) : Context A C :=
+    let '(froms, node, label, tos) := c in
+    (map (fun '(l, n) => (f (n, node, l), n)) froms, node, label, map (fun '(l, n) => (f (node, n, l), n)) tos).
+
+Lemma _rename_edge_label_correct : forall (A B C : Type) (f : LEdge B -> C) (ig1 ig2 : IG A B),
+    ig1 I== ig2
+    -> IG_gmap (fun c => _rename_edge_label f c) ig1 I== IG_gmap (fun c => _rename_edge_label f c) ig2.
+Proof.
+Admitted.
+
+
+
+
+
+
+
+
+
+
+
+
+
+
+
+
+
+
+
+
+
+
+
+
+(* Now, I try a fully new approach, where I look at what the paper has done *)
+
+(* Fact 2, for each graph h and each node v. there exists p l s an d g' such that (p v ö s) & g' = G *)
+
+Definition IG_equiv' {A B : Type} (ig1 ig2 : IG A B) : Prop :=
+    RG_equiv (IG_to_RG' ig1) (IG_to_RG' ig2).
+
+Notation "g1 I==' g2" := (IG_equiv' g1 g2) (at level 80).
+
+
+
+
+Lemma IG_match_rev_and : forall (A B : Type) (c : Context A B) (ig i : IG A B),
+    let '(froms, node, label, tos) := c in
+    IG_match node ig = (Some (froms, node, label, tos), i)
+    -> ig I==' (froms, node, label, tos) I& i.
+Proof.
+    intros. destruct_context c. intros.
+    simpl.
+    destruct (NatMap.mem node i) eqn:cond.
+    - exfalso. apply IG_match_removes_node in H as mat. apply mat.
+        unfold _key_In_IG. setoid_rewrite _In_labNodes_is_some_MapsTo.
+        apply MFacts.mem_in_iff in cond.
+        apply -> NatMap_In_exists_MapsTo_iff in cond.
+        destruct cond. destruct_context' x.
+        exists label'.
+        exists froms', tos'.
+        assumption.
+    
+    - unfold IG_match in H. destruct (NatMap.find node ig) eqn:found.
+        + destruct (_cleanSplit node c (NatMap.remove node ig)) eqn:split.
+            destruct_contextt c0.
+            inversion H. subst. clear H.
+            unfold _cleanSplit in split.
+            destruct_context' c.
+            inversion split. subst. clear split.
+
+            unfold IG_equiv'.
+            unfold RG_equiv. simpl. 
+            split; intros.
+            -- unfold _key_In_IG.
+                setoid_rewrite _updAdj_addSucc_does_not_change_IG_labNodes.
+                setoid_rewrite _updAdj_addPred_does_not_change_IG_labNodes.
+                setoid_rewrite _In_labNodes_is_some_MapsTo.
+
+                rewrite <- MFacts.find_mapsto_iff in found.
+                simpl. setoid_rewrite MFacts.add_mapsto_iff.
+                
+                bdestruct (node =? a).
+                ++ subst. firstorder.
+                    exists label, (filter (fun '(_, n) => negb (n =? a)) froms'), tos. firstorder.
+                ++ assert ((exists (other : A) (froms tos0 : Adj B), NatMap.MapsTo a (froms, other, tos0) ig)
+                                <-> (exists (other : A) (froms tos0 : Adj B), NatMap.MapsTo a (froms, other, tos0) (_updAdj (filter (fun '(_, n) => negb (n =? node)) tos) (fun (_ : B) (y : Context' A B) => _clearPred node y) (_updAdj (filter (fun '(_, n) => negb (n =? node)) froms') (fun (_ : B) (y : Context' A B) => _clearSucc node y) (NatMap.remove (elt:=Context' A B) node ig))))). {
+                                pose proof _updAdj_does_not_change_key_set.
+                                unfold _key_In_IG in H0.
+                                setoid_rewrite _In_labNodes_is_some_MapsTo in H0.
+                                setoid_rewrite H0.
+                                setoid_rewrite H0.
+                                setoid_rewrite MProps.F.remove_neq_mapsto_iff.
+                                - reflexivity.
+                                - assumption.
+                    }
+
+                    rewrite H0. clear H0. 
+                    split; intros.
+                    --- firstorder.
+                    --- firstorder.
+
+            -- admit. (* Edges (NMUUUUUUUCH harder) I have no theorems about IG_labEdges *) 
+        
+        + inversion H.
 
 Admitted.
 
 
 
-*)
 
 
+(* This thoof is finished unless IG_match_rev_and *)
+Theorem Erwig_Fact2 : forall (A B : Type) (ig : IG A B) (n : Node),
+    _key_In_IG n ig
+        -> exists froms label tos i, ig I==' (froms, n, label, tos) I& i.
+Proof.
+    intros.
+    destruct (IG_match n ig) eqn:mat. destruct m.
+    - destruct_context c. exists froms, label, tos, i.
+        apply IG_match_returns_node in mat as mat'.
+        subst.
+        apply (IG_match_rev_and _ _ (froms, node, label, tos)).
+        assumption.
 
+    - exfalso. unfold _key_In_IG in H. unfold IG_match in mat.
+        destruct (NatMap.find n ig) eqn:found.
+        + destruct (_cleanSplit n c (NatMap.remove n ig)). inversion mat.
+        + apply MFacts.not_find_in_iff in found.
+            setoid_rewrite _In_labNodes_is_some_MapsTo in H.
+            rewrite NatMap_In_exists_MapsTo_iff in found.
+            apply found.
+            destruct H.
+            destruct_eMapsTo H.
+            exists (efroms, x, etos).
+            assumption.
 
-
+Qed.
