src/algebraic/AG_theory.v
@@ -78,12 +78,12 @@ Qed.
 
 Ltac Proper_proof_automation := split; simpl in *; firstorder.
 
-Instance Proper_add {A : Type} : Proper ((@AG_equiv A) ==> AG_equiv ==> AG_equiv) AG_overlay.
+Instance Proper_overlay {A : Type} : Proper ((@AG_equiv A) ==> AG_equiv ==> AG_equiv) AG_overlay.
 Proof.
     Proper_proof_automation.
 Qed.
 
-Instance Proper_mul {A : Type} : Proper ((@AG_equiv A) ==> AG_equiv ==> AG_equiv) AG_connect.
+Instance Proper_connect {A : Type} : Proper ((@AG_equiv A) ==> AG_equiv ==> AG_equiv) AG_connect.
 Proof.
     Proper_proof_automation.
 Qed.
@@ -160,16 +160,6 @@ Proof.
     rewrite AG_overlay_Idempotence.
     reflexivity.
 Qed.
-
-
-
-
-
-
-
-
-
-
 
 
 
@@ -292,6 +282,7 @@ Qed.
 
 
 
+
 Lemma _consolidation_fold_right_preserves_nodes : forall (l : list (NatSet.t)) y,
     (exists x, In x l /\ NatSet.In y x) <-> (In y (fold_right (fun next acc => NatSet.elements next ++ NatList_filterOutOf next acc) nil l)) .
 Proof. 
@@ -386,19 +377,99 @@ Qed.
 
 
 
-
-
-
 (* Here are attempts at specifying which elements are in BFS and in which order *)
 
 
-(* About what is included *)
-Theorem AG_BFS_path : forall (nodes : list nat) (ag : AG nat) x,
-    In x (AG_BFS nodes ag)
-        -> exists y, In y nodes /\ RG_existsPath y x (AG_to_RG ag).
+
+
+Lemma AG_nodeAmount_empty :
+    AG_nodeAmount AG_empty = 0.
+Proof.
+    unfold AG_nodeAmount. reflexivity.
+Qed.
+
+Lemma NatSet_emptyElements : forall (nodes : list Node),
+    NatSet.elements (NatSet.inter (NatSet_fromList nodes) NatSet.empty) = [].
 Proof.
     intros.
+    apply SProps.MP.elements_Empty. apply SProps.MP.empty_inter_2. apply NatSet.empty_spec.
+Qed.
+
+
+Require Import Relation_Operators.
+
+Lemma if_same_result : forall (A : Type) (a : A) (b : bool),
+    (if b then a else a) = a.
+Proof.
+    intros. destruct b. reflexivity. reflexivity.
+Qed.
+
+Require Import GraphVerification.src.util.util.
+Require Import Arith.
+
+(* About what is included, can also add that every node that has a path is i the result *)
+Theorem AG_BFS_path : forall (nodes : list nat) (ag : AG nat) x,
+    In x (AG_BFS nodes ag)
+        -> In x nodes \/ exists y, In y nodes /\ RG_existsPath y x (AG_to_RG ag). 
+Proof.
+    intros. induction ag.
+    - exfalso. unfold AG_BFS in H. simpl in H. rewrite NatSet_emptyElements in H. destruct (NatSet.equal (NatSet.inter (NatSet_fromList nodes) NatSet.empty)
+(NatSet.union (NatSet.inter (NatSet_fromList nodes) NatSet.empty) NatSet.empty)).
+        ++ simpl in H. inversion H.
+        ++ simpl in H. inversion H.
+    - left. 
+        unfold AG_BFS in H.
+        apply _consolidation_fold_right_preserves_nodes in H.
+        destruct H. destruct H.
+        simpl in H. destruct H.
+        + destruct (existsb (Nat.eqb a) nodes) eqn:has.
+            -- admit.
+            -- exfalso. admit. 
+        + rewrite if_same_result in H.
+            destruct (NatSet.equal (NatSet.inter (NatSet_fromList nodes) (NatSet.singleton a)) (NatSet.union (NatSet.inter (NatSet_fromList nodes) (NatSet.singleton a)) NatSet.empty)).
+            -- inversion H.
+            -- simpl in *. destruct H. 
+                ++ subst. apply SProps.MP.FM.empty_iff in H0. inversion H0.
+                ++ inversion H.
+    - unfold AG_BFS in H.
+        apply _consolidation_fold_right_preserves_nodes in H.
+        destruct H. destruct H.
+        simpl in H. destruct H.
+
 Admitted.
+
+
+
+
+
+Theorem AG_BFS_path' : forall (nodes : list nat) (ag : AG nat) x,
+    In x (AG_BFS nodes ag)
+        -> In x nodes \/ exists y, In y nodes /\ RG_existsPath y x (AG_to_RG ag). 
+Proof.
+    intros.  
+    unfold AG_BFS in H.
+    apply _consolidation_fold_right_preserves_nodes in H.
+    destruct H. destruct H.
+    induction ag.
+    - admit.
+    - admit.
+    - simpl in H. destruct H.
+        + left. admit.
+        + destruct (NatSet.equal (NatSet.inter (NatSet_fromList nodes) (NatSet.union (AG_nodeSet ag1) (AG_nodeSet ag2)))
+(NatSet.union (NatSet.inter (NatSet_fromList nodes) (NatSet.union (AG_nodeSet ag1) (AG_nodeSet ag2)))
+(NatSet.union (_singleStep (NatSet.inter (NatSet_fromList nodes) (NatSet.union (AG_nodeSet ag1) (AG_nodeSet ag2))) ag1)
+(_singleStep (NatSet.inter (NatSet_fromList nodes) (NatSet.union (AG_nodeSet ag1) (AG_nodeSet ag2))) ag2)))).
+            -- inversion H.
+            -- unfold RG_existsPath.
+                 (* Now that I think of how RG_existsPath would even be split up, I don't really know how this could be continued..... hmmm. There is the problem, that if one does a zig zag from ag1 to ag2. combining the two IH is not really enough, right? *)
+            
+            
+            
+
+Admitted.
+
+
+
 
 
 
